---
title: "Cholera SEIR equation"
author: "Jong-Hoon Kim"
date: "2023-12-29"
categories: [cholera, sub-Saharan Africa]
image: "sample_figure.png"
editor_options: 
  chunk_output_type: console
---

```{r setup, include=FALSE}
knitr::opts_chunk$set(warning=FALSE, message=FALSE) 
```

### Cholera SEIR equation

\begin{align} 
\lambda_p &= \frac{\beta(I_1+I_2+ (1-\psi_1)  (I_1^O+I_2^O)+ (1-\psi_2) (I_1^T+I_2^T))}{N}\\ 
\mathrm{d}S/\mathrm{d}t &= - (\lambda_p+\lambda_w)S + 2 \omega R_2 \\ 
\mathrm{d}E_1/\mathrm{d}t &= (\lambda_p+\lambda_w)S - 2\epsilon E_1\\
\mathrm{d}E_2/\mathrm{d}t &= 2\epsilon E_1 - 2\epsilon E_2 \\
\mathrm{d}I_1/\mathrm{d}t &= 2 (1-\theta) \epsilon E_2 - 2 \gamma I_1 \\
\mathrm{d}I_2/\mathrm{d}t &= 2 \gamma I_1 - 2 \gamma I_2 \\
\mathrm{d}A_1/\mathrm{d}t &= 2 \theta \epsilon E_2 - 2 \gamma A_1 \\
\mathrm{d}A_2/\mathrm{d}t &= 2 \gamma A_1 - 2 \gamma A_2 \\
\mathrm{d}R_1/\mathrm{d}t &= 2 \gamma (I_2 + A_2) - 2 \omega R_1 \\
\mathrm{d}R_2/\mathrm{d}t &= 2 \omega (R_1 - R_2) \\

\mathrm{d}S^O/\mathrm{d}t &= - (\lambda_p+\lambda_w)S^O + 2 \omega R_2^O + 2 \omega_V O_2 \\ 
\mathrm{d}O_1/\mathrm{d}t &= + v^O S - 2 \omega_V O_1 - (\lambda_p+\lambda_w)(1-\chi^O) O_1 \\
\mathrm{d}O_2/\mathrm{d}t &= + 2 \omega_V O_1 - 2 \omega_V O_2 - (\lambda_p+\lambda_w)(1-\chi^O) O_2 \\
\mathrm{d}E_1^O/\mathrm{d}t &= (\lambda_p+\lambda_w) ((1-\chi^O)(O_1+O_2) + S^O) + v^O E_1 - v^T E_1^O - 2\epsilon E_1^O\\
\mathrm{d}E_2^O/\mathrm{d}t &= 2\epsilon E_1^O - 2\epsilon E_2^O + v^O E_2 - v^T E_2^O\\
\mathrm{d}I_1^O/\mathrm{d}t &= 2 (1-\theta) \epsilon E_2^O - 2 \gamma I_1^O \\
\mathrm{d}I_2^O/\mathrm{d}t &= 2 \gamma I_1^O - 2 \gamma I_2^O \\
\mathrm{d}A_1^O/\mathrm{d}t &= 2 \theta \epsilon E_2^O - 2 \gamma A_1^O + v^O A_1 - v^T A_1^O\\
\mathrm{d}A_2^O/\mathrm{d}t &= 2 \gamma A_1^O - 2 \gamma A_2^O + v^O A_2 - v^T A_2^O\\
\mathrm{d}R_1^O/\mathrm{d}t &= 2 \gamma (I_2^O + A_2^O) - 2 \omega R_1^O + v^O R_1 - v^T R_1^O\\
\mathrm{d}R_2^O/\mathrm{d}t &= 2 \omega (R_1^O - R_2^O) + v^O R_2 - v^T R_2^O\\

\mathrm{d}S^T/\mathrm{d}t &= - (\lambda_p+\lambda_w)S^T + 2 \omega R_2^T + 2 \omega_V T_2 \\ 
\mathrm{d}T_1/\mathrm{d}t &= + v S^O - 2 \omega_V T_1 - (\lambda_p+\lambda_w)(1-\chi^T) T_1\\
\mathrm{d}T_2/\mathrm{d}t &= + 2 \omega_V T_1 - 2 \omega_V T_2 - (\lambda_p+\lambda_w)(1-\chi^T) T_2\\
\mathrm{d}E_1^T/\mathrm{d}t &= (\lambda_p+\lambda_w)(S^T + (1-\chi^T)(T_1+T_2)) - 
  2\epsilon E_1^T + v^T E_1^O\\
\mathrm{d}E_2^T/\mathrm{d}t &= 2\epsilon E_1^T - 2\epsilon E_2^T + v^T E_2^O\\
\mathrm{d}I_1^T/\mathrm{d}t &= 2 (1-\theta) \epsilon E_2^T - 2 \gamma I_1^T\\
\mathrm{d}I_2^T/\mathrm{d}t &= 2 \gamma I_1^T - 2 \gamma I_2^T \\
\mathrm{d}A_1^T/\mathrm{d}t &= 2 \theta \epsilon E_2^T - 2 \gamma A_1^T + v^T A_1^O \\
\mathrm{d}A_2^T/\mathrm{d}t &= 2 \gamma A_1^T - 2 \gamma A_2^T + v^T A_2^O \\
\mathrm{d}R_1^T/\mathrm{d}t &= 2 \gamma (I_2^T + A_2^T) - 2 \omega R_1^T + v^T R_1^O \\
\mathrm{d}R_2^T/\mathrm{d}t &= 2 \omega (R_1^T - R_2^T) + v^T R_2^O \\

\end{align}
